<?xml version="1.0" encoding="UTF-8"?>
<rdf:RDF
	xmlns="http://vocab.linkeddata.es/datosabiertos/def/sector-publico/agenda-municipal#"
	xmlns:dc="http://purl.org/dc/elements/1.1/"
	xmlns:ns="http://www.w3.org/2003/06/sw-vocab-status/ns#"
	xmlns:dbo="http://dbpedia.org/ontology/"
	xmlns:org="https://www.w3.org/TR/vocab-org/"
	xmlns:owl="http://www.w3.org/2002/07/owl#"
	xmlns:rdf="http://www.w3.org/1999/02/22-rdf-syntax-ns#"
	xmlns:xml="http://www.w3.org/XML/1998/namespace"
	xmlns:xsd="http://www.w3.org/2001/XMLSchema#"
	xmlns:foaf="http://xmlns.com/foaf/0.1/"
	xmlns:rdfs="http://www.w3.org/2000/01/rdf-schema#"
	xmlns:skos="http://www.w3.org/2004/02/skos/core#"
	xmlns:esadm="http://vocab.linkeddata.es/datosabiertos/def/sector-publico/territorio#"
	xmlns:orges="http://vocab.linkeddata.es/datosabiertos/def/sector-publico/organizacion#"
	xmlns:skos1="http://www.w3.org/2008/05/skos#"
	xmlns:terms="http://purl.org/dc/terms/"
	xmlns:schema="https://schema.org/"
	xmlns:esequip="http://vocab.linkeddata.es/datosabiertos/def/urbanismo-infraestructuras/equipamiento#">

<rdf:Description rdf:about="http://vocab.linkeddata.es/datosabiertos/def/sector-publico/agenda-municipal#">
	<rdf:type rdf:resource="http://www.w3.org/2002/07/owl#Ontology"/>
	<owl:versionIRI rdf:resource="http://vocab.linkeddata.es/datosabiertos/def/sector-publico/agenda-municipal#"/>
	<dc:contributor xml:lang="es">Red.es</dc:contributor>
	<terms:creator rdf:datatype="http://www.w3.org/2001/XMLSchema#string">Paola Espinoza Arias (Ontology Engineering Group - Universidad Politécnica de Madrid)</terms:creator>
	<rdfs:comment xml:lang="es">sta versión ha sido generada dentro del contexto del proyecto "Plataforma de gobierno abierto, colaborativa e interoperable" en el que participan los ayuntamientos de Madrid, Zaragoza, Santiago de Compostela y A Coruña.   

En esta versión se han clases y propiedades de acuerdo a los requisitos y glosario de conceptos propuestos en la reuni'on del 22/03/2019</rdfs:comment>
	<dc:title xml:lang="en">Vocabulary for the representation of data on the events that take place within the municipal agenda and their participants</dc:title>
	<terms:license rdf:datatype="http://www.w3.org/2001/XMLSchema#string">https://creativecommons.org/licenses/by/4.0</terms:license>
	<dc:contributor xml:lang="es">Servicio de Informática - Ayuntamiento de Santiago de Compostela</dc:contributor>
	<dc:identifier xml:lang="es">http://vocab.linkeddata.es/datosabiertos/def/sector-publico/agenda-municipal</dc:identifier>
	<dc:title xml:lang="es">Vocabulario para la representación de datos sobre los eventos que se realizan dentro de la agenda municipal y sus asistentes, convocantes y titulares</dc:title>
	<terms:issued xml:lang="es">2019-03-22</terms:issued>
	<dc:creator rdf:datatype="http://www.w3.org/2001/XMLSchema#string">Oscar Corcho (Ontology Engineering Group - Universidad Politécnica de Madrid, Localidata)</dc:creator>
	<dc:contributor xml:lang="es">Servicio de Acceso a la Información - Ayuntamiento de Madrid</dc:contributor>
	<dc:contributor xml:lang="es">Oficina Técnica de Participación, Transparencia y Gobierno Abierto - Ayuntamiento de Zaragoza</dc:contributor>
	<terms:hasFormat xml:lang="es">http://vocab.linkeddata.es/datosabiertos/def/sector-publico/agenda-municipal.ttl</terms:hasFormat>
	<dc:contributor xml:lang="es">Servicio de Innovación y Desarrollo Tecnológico - Ayuntamiento de A Coruña</dc:contributor>
	<dc:creator rdf:datatype="http://www.w3.org/2001/XMLSchema#string">Edna Ruckhaus (Ontology Engineering Group - Universidad Politécnica de Madrid)</dc:creator>
	<dc:rights rdf:datatype="http://www.w3.org/2001/XMLSchema#string">Creative Commons Attribution 4.0 International (CC BY 4.0)</dc:rights>
</rdf:Description>
<!--  -->
<!--  -->
<!-- ################################################################# -->
<!-- # -->
<!-- #    Annotation properties -->
<!-- # -->
<!-- ################################################################# -->
<!--  -->
<!--  -->
<!-- http://purl.org/dc/elements/1.1/contributor -->

<rdf:Description rdf:about="http://purl.org/dc/elements/1.1/contributor">
	<rdf:type rdf:resource="http://www.w3.org/2002/07/owl#AnnotationProperty"/>
</rdf:Description>
<!--  -->
<!-- http://purl.org/dc/elements/1.1/creator -->

<rdf:Description rdf:about="http://purl.org/dc/elements/1.1/creator">
	<rdf:type rdf:resource="http://www.w3.org/2002/07/owl#AnnotationProperty"/>
</rdf:Description>
<!--  -->
<!-- http://purl.org/dc/elements/1.1/date -->

<rdf:Description rdf:about="http://purl.org/dc/elements/1.1/date">
	<rdf:type rdf:resource="http://www.w3.org/2002/07/owl#AnnotationProperty"/>
</rdf:Description>
<!--  -->
<!-- http://purl.org/dc/elements/1.1/description -->

<rdf:Description rdf:about="http://purl.org/dc/elements/1.1/description">
	<rdf:type rdf:resource="http://www.w3.org/2002/07/owl#AnnotationProperty"/>
</rdf:Description>
<!--  -->
<!-- http://purl.org/dc/elements/1.1/identifier -->

<rdf:Description rdf:about="http://purl.org/dc/elements/1.1/identifier">
	<rdf:type rdf:resource="http://www.w3.org/2002/07/owl#AnnotationProperty"/>
</rdf:Description>
<!--  -->
<!-- http://purl.org/dc/elements/1.1/relation -->

<rdf:Description rdf:about="http://purl.org/dc/elements/1.1/relation">
	<rdf:type rdf:resource="http://www.w3.org/2002/07/owl#AnnotationProperty"/>
</rdf:Description>
<!--  -->
<!-- http://purl.org/dc/elements/1.1/rights -->

<rdf:Description rdf:about="http://purl.org/dc/elements/1.1/rights">
	<rdf:type rdf:resource="http://www.w3.org/2002/07/owl#AnnotationProperty"/>
</rdf:Description>
<!--  -->
<!-- http://purl.org/dc/elements/1.1/title -->

<rdf:Description rdf:about="http://purl.org/dc/elements/1.1/title">
	<rdf:type rdf:resource="http://www.w3.org/2002/07/owl#AnnotationProperty"/>
</rdf:Description>
<!--  -->
<!-- http://purl.org/dc/terms/abstract -->

<rdf:Description rdf:about="http://purl.org/dc/terms/abstract">
	<rdf:type rdf:resource="http://www.w3.org/2002/07/owl#AnnotationProperty"/>
	<rdfs:subPropertyOf rdf:resource="http://purl.org/dc/elements/1.1/description"/>
</rdf:Description>
<!--  -->
<!-- http://purl.org/dc/terms/accessRights -->

<rdf:Description rdf:about="http://purl.org/dc/terms/accessRights">
	<rdf:type rdf:resource="http://www.w3.org/2002/07/owl#AnnotationProperty"/>
	<rdfs:subPropertyOf rdf:resource="http://purl.org/dc/elements/1.1/rights"/>
</rdf:Description>
<!--  -->
<!-- http://purl.org/dc/terms/alternative -->

<rdf:Description rdf:about="http://purl.org/dc/terms/alternative">
	<rdf:type rdf:resource="http://www.w3.org/2002/07/owl#AnnotationProperty"/>
	<rdfs:subPropertyOf rdf:resource="http://purl.org/dc/elements/1.1/title"/>
</rdf:Description>
<!--  -->
<!-- http://purl.org/dc/terms/bibliographicCitation -->

<rdf:Description rdf:about="http://purl.org/dc/terms/bibliographicCitation">
	<rdf:type rdf:resource="http://www.w3.org/2002/07/owl#AnnotationProperty"/>
	<rdfs:subPropertyOf rdf:resource="http://purl.org/dc/elements/1.1/identifier"/>
</rdf:Description>
<!--  -->
<!-- http://purl.org/dc/terms/creator -->

<rdf:Description rdf:about="http://purl.org/dc/terms/creator">
	<rdf:type rdf:resource="http://www.w3.org/2002/07/owl#AnnotationProperty"/>
	<rdfs:subPropertyOf rdf:resource="http://purl.org/dc/elements/1.1/creator"/>
</rdf:Description>
<!--  -->
<!-- http://purl.org/dc/terms/description -->

<rdf:Description rdf:about="http://purl.org/dc/terms/description">
	<rdf:type rdf:resource="http://www.w3.org/2002/07/owl#AnnotationProperty"/>
	<rdfs:subPropertyOf rdf:resource="http://purl.org/dc/elements/1.1/description"/>
</rdf:Description>
<!--  -->
<!-- http://purl.org/dc/terms/hasFormat -->

<rdf:Description rdf:about="http://purl.org/dc/terms/hasFormat">
	<rdf:type rdf:resource="http://www.w3.org/2002/07/owl#AnnotationProperty"/>
	<terms:hasVersion rdf:resource="http://dublincore.org/usage/terms/history/#hasFormat-003"/>
	<rdfs:comment xml:lang="en">A related resource that is substantially the same as the pre-existing described resource, but in another format.</rdfs:comment>
	<rdfs:isDefinedBy rdf:resource="http://purl.org/dc/terms/"/>
	<rdfs:label xml:lang="en">Has Format</rdfs:label>
	<skos:note xml:lang="en">This term is intended to be used with non-literal values as defined in the DCMI Abstract Model (http://dublincore.org/documents/abstract-model/).  As of December 2007, the DCMI Usage Board is seeking a way to express this intention with a formal range declaration.</skos:note>
	<rdfs:subPropertyOf rdf:resource="http://purl.org/dc/elements/1.1/relation"/>
	<rdfs:subPropertyOf rdf:resource="http://purl.org/dc/terms/relation"/>
</rdf:Description>
<!--  -->
<!-- http://purl.org/dc/terms/hasVersion -->

<rdf:Description rdf:about="http://purl.org/dc/terms/hasVersion">
	<rdf:type rdf:resource="http://www.w3.org/2002/07/owl#AnnotationProperty"/>
</rdf:Description>
<!--  -->
<!-- http://purl.org/dc/terms/identifier -->

<rdf:Description rdf:about="http://purl.org/dc/terms/identifier">
	<rdf:type rdf:resource="http://www.w3.org/2002/07/owl#AnnotationProperty"/>
	<rdfs:subPropertyOf rdf:resource="http://purl.org/dc/elements/1.1/identifier"/>
</rdf:Description>
<!--  -->
<!-- http://purl.org/dc/terms/issued -->

<rdf:Description rdf:about="http://purl.org/dc/terms/issued">
	<rdf:type rdf:resource="http://www.w3.org/2002/07/owl#AnnotationProperty"/>
	<terms:hasVersion rdf:resource="http://dublincore.org/usage/terms/history/#issued-003"/>
	<rdfs:comment xml:lang="en">Date of formal issuance (e.g., publication) of the resource.</rdfs:comment>
	<rdfs:isDefinedBy rdf:resource="http://purl.org/dc/terms/"/>
	<rdfs:label xml:lang="en">Date Issued</rdfs:label>
	<rdfs:subPropertyOf rdf:resource="http://purl.org/dc/elements/1.1/date"/>
</rdf:Description>
<!--  -->
<!-- http://purl.org/dc/terms/license -->

<rdf:Description rdf:about="http://purl.org/dc/terms/license">
	<rdf:type rdf:resource="http://www.w3.org/2002/07/owl#AnnotationProperty"/>
	<rdfs:subPropertyOf rdf:resource="http://purl.org/dc/elements/1.1/rights"/>
</rdf:Description>
<!--  -->
<!-- http://purl.org/dc/terms/modified -->

<rdf:Description rdf:about="http://purl.org/dc/terms/modified">
	<rdf:type rdf:resource="http://www.w3.org/2002/07/owl#AnnotationProperty"/>
</rdf:Description>
<!--  -->
<!-- http://purl.org/dc/terms/relation -->

<rdf:Description rdf:about="http://purl.org/dc/terms/relation">
	<rdf:type rdf:resource="http://www.w3.org/2002/07/owl#AnnotationProperty"/>
</rdf:Description>
<!--  -->
<!-- http://purl.org/dc/terms/rights -->

<rdf:Description rdf:about="http://purl.org/dc/terms/rights">
	<rdf:type rdf:resource="http://www.w3.org/2002/07/owl#AnnotationProperty"/>
	<rdfs:subPropertyOf rdf:resource="http://purl.org/dc/elements/1.1/rights"/>
</rdf:Description>
<!--  -->
<!-- http://purl.org/dc/terms/tableOfContents -->

<rdf:Description rdf:about="http://purl.org/dc/terms/tableOfContents">
	<rdf:type rdf:resource="http://www.w3.org/2002/07/owl#AnnotationProperty"/>
	<rdfs:subPropertyOf rdf:resource="http://purl.org/dc/elements/1.1/description"/>
</rdf:Description>
<!--  -->
<!-- http://purl.org/dc/terms/title -->

<rdf:Description rdf:about="http://purl.org/dc/terms/title">
	<rdf:type rdf:resource="http://www.w3.org/2002/07/owl#AnnotationProperty"/>
	<rdfs:subPropertyOf rdf:resource="http://purl.org/dc/elements/1.1/title"/>
</rdf:Description>
<!--  -->
<!-- http://www.w3.org/2003/06/sw-vocab-status/ns#term_status -->

<rdf:Description rdf:about="http://www.w3.org/2003/06/sw-vocab-status/ns#term_status">
	<rdf:type rdf:resource="http://www.w3.org/2002/07/owl#AnnotationProperty"/>
</rdf:Description>
<!--  -->
<!-- http://www.w3.org/2004/02/skos/core#definition -->

<rdf:Description rdf:about="http://www.w3.org/2004/02/skos/core#definition">
	<rdf:type rdf:resource="http://www.w3.org/2002/07/owl#AnnotationProperty"/>
</rdf:Description>
<!--  -->
<!-- http://www.w3.org/2004/02/skos/core#example -->

<rdf:Description rdf:about="http://www.w3.org/2004/02/skos/core#example">
	<rdf:type rdf:resource="http://www.w3.org/2002/07/owl#AnnotationProperty"/>
</rdf:Description>
<!--  -->
<!-- http://www.w3.org/2004/02/skos/core#note -->

<rdf:Description rdf:about="http://www.w3.org/2004/02/skos/core#note">
	<rdf:type rdf:resource="http://www.w3.org/2002/07/owl#AnnotationProperty"/>
</rdf:Description>
<!--  -->
<!-- http://www.w3.org/2004/02/skos/core#scopeNote -->

<rdf:Description rdf:about="http://www.w3.org/2004/02/skos/core#scopeNote">
	<rdf:type rdf:resource="http://www.w3.org/2002/07/owl#AnnotationProperty"/>
</rdf:Description>
<!--  -->
<!-- http://www.w3.org/2008/05/skos#definition -->

<rdf:Description rdf:about="http://www.w3.org/2008/05/skos#definition">
	<rdf:type rdf:resource="http://www.w3.org/2002/07/owl#AnnotationProperty"/>
</rdf:Description>
<!--  -->
<!--  -->
<!--  -->
<!-- ################################################################# -->
<!-- # -->
<!-- #    Object Properties -->
<!-- # -->
<!-- ################################################################# -->
<!--  -->
<!--  -->
<!-- http://schema.org/location -->

<rdf:Description rdf:about="http://schema.org/location">
	<rdf:type rdf:resource="http://www.w3.org/2002/07/owl#ObjectProperty"/>
	<rdfs:domain rdf:resource="http://schema.org/Event"/>
	<rdfs:range rdf:resource="http://schema.org/Place"/>
	<rdfs:comment>The location of for example where the event is happening, an organization is located, or where an action takes place.</rdfs:comment>
	<rdfs:isDefinedBy>https://schema.org/location</rdfs:isDefinedBy>
	<rdfs:label>location</rdfs:label>
</rdf:Description>
<!--  -->
<!-- http://schema.org/name -->

<rdf:Description rdf:about="http://schema.org/name">
	<rdf:type rdf:resource="http://www.w3.org/2002/07/owl#ObjectProperty"/>
	<rdfs:subPropertyOf rdf:resource="rdfs:label"/>
	<rdfs:domain rdf:nodeID="genid1"/>
</rdf:Description>

<rdf:Description rdf:nodeID="genid1">
	<rdf:type rdf:resource="http://www.w3.org/2002/07/owl#Class"/>
	<owl:unionOf rdf:nodeID="genid2"/>
</rdf:Description>

<rdf:Description rdf:nodeID="genid2">
	<rdf:type rdf:resource="http://www.w3.org/1999/02/22-rdf-syntax-ns#List"/>
	<rdf:first rdf:resource="http://schema.org/Thing"/>
	<rdf:rest rdf:resource="http://www.w3.org/1999/02/22-rdf-syntax-ns#nil"/>
</rdf:Description>

<rdf:Description rdf:about="http://schema.org/name">
	<rdfs:range rdf:resource="http://schema.org/Text"/>
</rdf:Description>
<!--  -->
<!-- http://schema.org/subEvent -->

<rdf:Description rdf:about="http://schema.org/subEvent">
	<rdf:type rdf:resource="http://www.w3.org/2002/07/owl#ObjectProperty"/>
	<owl:inverseOf rdf:resource="http://schema.org/superEvent"/>
	<rdfs:domain rdf:resource="http://schema.org/Event"/>
	<rdfs:range rdf:resource="http://schema.org/Event"/>
	<rdfs:comment xml:lang="en">An Event that is part of this event. For example, a conference event includes many presentations, each of which is a subEvent of the conference.</rdfs:comment>
	<rdfs:isDefinedBy rdf:resource="https://schema.org/subEvent"/>
	<rdfs:label xml:lang="en">subEvent</rdfs:label>
</rdf:Description>
<!--  -->
<!-- http://schema.org/superEvent -->

<rdf:Description rdf:about="http://schema.org/superEvent">
	<rdf:type rdf:resource="http://www.w3.org/2002/07/owl#ObjectProperty"/>
	<rdfs:domain rdf:resource="http://schema.org/Event"/>
	<rdfs:range rdf:resource="http://schema.org/Event"/>
	<rdfs:comment xml:lang="en">An event that this event is a part of. For example, a collection of individual music performances might each have a music festival as their superEvent.</rdfs:comment>
	<rdfs:isDefinedBy xml:lang="en">https://schema.org/superEvent</rdfs:isDefinedBy>
	<rdfs:label xml:lang="en">superEvent</rdfs:label>
</rdf:Description>
<!--  -->
<!-- http://vocab.linkeddata.es/datosabiertos/def/sector-publico/agenda-municipal##ambitoEvento -->

<rdf:Description rdf:about="http://vocab.linkeddata.es/datosabiertos/def/sector-publico/agenda-municipal##ambitoEvento">
	<rdf:type rdf:resource="http://www.w3.org/2002/07/owl#ObjectProperty"/>
	<rdfs:domain rdf:resource="http://vocab.linkeddata.es/datosabiertos/def/sector-publico/agenda-municipal##Evento"/>
	<rdfs:range rdf:resource="http://dbpedia.org/ontology/GovernmentalAdministrativeRegion"/>
	<rdfs:comment xml:lang="en">Territorial scope of an event.</rdfs:comment>
	<rdfs:comment xml:lang="es">Ámbito territorial de un evento.</rdfs:comment>
	<rdfs:label xml:lang="en">territorial scope</rdfs:label>
	<rdfs:label xml:lang="es">ámbito territorial</rdfs:label>
</rdf:Description>
<!--  -->
<!-- http://vocab.linkeddata.es/datosabiertos/def/sector-publico/agenda-municipal##canal -->

<rdf:Description rdf:about="http://vocab.linkeddata.es/datosabiertos/def/sector-publico/agenda-municipal##canal">
	<rdf:type rdf:resource="http://www.w3.org/2002/07/owl#ObjectProperty"/>
	<rdfs:domain rdf:resource="http://vocab.linkeddata.es/datosabiertos/def/sector-publico/agenda-municipal##Evento"/>
	<rdfs:range rdf:nodeID="genid3"/>
</rdf:Description>

<rdf:Description rdf:nodeID="genid3">
	<owl:intersectionOf rdf:nodeID="genid6"/>
</rdf:Description>

<rdf:Description rdf:nodeID="genid6">
	<rdf:type rdf:resource="http://www.w3.org/1999/02/22-rdf-syntax-ns#List"/>
	<rdf:first rdf:resource="http://www.w3.org/2004/02/skos/core#Concept"/>
	<rdf:rest rdf:nodeID="genid4"/>
</rdf:Description>

<rdf:Description rdf:nodeID="genid4">
	<rdf:type rdf:resource="http://www.w3.org/1999/02/22-rdf-syntax-ns#List"/>
	<rdf:first rdf:nodeID="genid5"/>
</rdf:Description>

<rdf:Description rdf:nodeID="genid5">
	<rdf:type rdf:resource="http://www.w3.org/2002/07/owl#Restriction"/>
	<owl:onProperty rdf:resource="http://www.w3.org/2004/02/skos/core#inScheme"/>
	<owl:hasValue rdf:resource="http://vocab.linkeddata.es/datosabiertos/kos/sector-publico/agenda-municipal/canal"/>
</rdf:Description>

<rdf:Description rdf:nodeID="genid4">
	<rdf:rest rdf:resource="http://www.w3.org/1999/02/22-rdf-syntax-ns#nil"/>
</rdf:Description>

<rdf:Description rdf:nodeID="genid3">
	<rdf:type rdf:resource="http://www.w3.org/2002/07/owl#Class"/>
</rdf:Description>

<rdf:Description rdf:about="http://vocab.linkeddata.es/datosabiertos/def/sector-publico/agenda-municipal##canal">
	<rdfs:comment xml:lang="en">Means for the realization of the event: face-to-face or online.</rdfs:comment>
	<rdfs:comment xml:lang="es">Medio de realización del evento: presencial o en línea.</rdfs:comment>
	<rdfs:isDefinedBy>http://vocab.linkeddata.es/datosabiertos/def/sector-publico/agenda-municipal</rdfs:isDefinedBy>
	<rdfs:label xml:lang="es">canal</rdfs:label>
	<rdfs:label xml:lang="en">channel</rdfs:label>
</rdf:Description>
<!--  -->
<!-- http://vocab.linkeddata.es/datosabiertos/def/sector-publico/agenda-municipal##documentacion -->

<rdf:Description rdf:about="http://vocab.linkeddata.es/datosabiertos/def/sector-publico/agenda-municipal##documentacion">
	<rdf:type rdf:resource="http://www.w3.org/2002/07/owl#ObjectProperty"/>
	<rdfs:domain rdf:resource="http://vocab.linkeddata.es/datosabiertos/def/sector-publico/agenda-municipal##Evento"/>
	<rdfs:range rdf:resource="http://vocab.linkeddata.es/datosabiertos/def/sector-publico/agenda-municipal##Documentacion"/>
	<rdfs:comment xml:lang="es">Asociación con la documentación como actas, mociones, vídeos.</rdfs:comment>
	<rdfs:comment xml:lang="en">Association with documentation such as minutes, motions, videos.</rdfs:comment>
	<rdfs:isDefinedBy>http://vocab.linkeddata.es/datosabiertos/def/sector-publico/agenda-municipal</rdfs:isDefinedBy>
	<rdfs:label xml:lang="es">asociado con</rdfs:label>
	<rdfs:label xml:lang="en">associated with</rdfs:label>
</rdf:Description>
<!--  -->
<!-- http://vocab.linkeddata.es/datosabiertos/def/sector-publico/agenda-municipal##evento -->

<rdf:Description rdf:about="http://vocab.linkeddata.es/datosabiertos/def/sector-publico/agenda-municipal##evento">
	<rdf:type rdf:resource="http://www.w3.org/2002/07/owl#ObjectProperty"/>
	<owl:inverseOf rdf:resource="http://vocab.linkeddata.es/datosabiertos/def/sector-publico/agenda-municipal##rolIntegrante"/>
	<rdfs:domain rdf:resource="http://vocab.linkeddata.es/datosabiertos/def/sector-publico/agenda-municipal##RolIntegranteEvento"/>
	<rdfs:range rdf:resource="http://vocab.linkeddata.es/datosabiertos/def/sector-publico/agenda-municipal##Evento"/>
	<rdfs:comment xml:lang="en">Event in which a member participates with a role.</rdfs:comment>
	<rdfs:comment xml:lang="es">Evento en el que participa un integrante con un rol.</rdfs:comment>
	<rdfs:isDefinedBy>http://vocab.linkeddata.es/datosabiertos/def/sector-publico/agenda-municipal</rdfs:isDefinedBy>
	<rdfs:label xml:lang="es">event</rdfs:label>
	<rdfs:label xml:lang="en">evento</rdfs:label>
</rdf:Description>
<!--  -->
<!-- http://vocab.linkeddata.es/datosabiertos/def/sector-publico/agenda-municipal##integra -->

<rdf:Description rdf:about="http://vocab.linkeddata.es/datosabiertos/def/sector-publico/agenda-municipal##integra">
	<rdf:type rdf:resource="http://www.w3.org/2002/07/owl#ObjectProperty"/>
	<rdfs:domain rdf:resource="http://vocab.linkeddata.es/datosabiertos/def/sector-publico/agenda-municipal##RolIntegranteEvento"/>
	<rdfs:range rdf:resource="http://xmlns.com/foaf/0.1/Agent"/>
	<rdfs:comment xml:lang="es">El integrante de un evento con un cierto rol.</rdfs:comment>
	<rdfs:comment xml:lang="en">The member of an event with a certain role.</rdfs:comment>
	<rdfs:isDefinedBy>http://vocab.linkeddata.es/datosabiertos/def/sector-publico/agenda-municipal</rdfs:isDefinedBy>
	<rdfs:label xml:lang="es">integra</rdfs:label>
	<rdfs:label xml:lang="en">integrates</rdfs:label>
</rdf:Description>
<!--  -->
<!-- http://vocab.linkeddata.es/datosabiertos/def/sector-publico/agenda-municipal##rol -->

<rdf:Description rdf:about="http://vocab.linkeddata.es/datosabiertos/def/sector-publico/agenda-municipal##rol">
	<rdf:type rdf:resource="http://www.w3.org/2002/07/owl#ObjectProperty"/>
	<rdfs:domain rdf:resource="http://vocab.linkeddata.es/datosabiertos/def/sector-publico/agenda-municipal##RolIntegranteEvento"/>
	<rdfs:range rdf:nodeID="genid7"/>
</rdf:Description>

<rdf:Description rdf:nodeID="genid7">
	<owl:intersectionOf rdf:nodeID="genid10"/>
</rdf:Description>

<rdf:Description rdf:nodeID="genid10">
	<rdf:type rdf:resource="http://www.w3.org/1999/02/22-rdf-syntax-ns#List"/>
	<rdf:first rdf:resource="http://www.w3.org/2004/02/skos/core#Concept"/>
	<rdf:rest rdf:nodeID="genid8"/>
</rdf:Description>

<rdf:Description rdf:nodeID="genid8">
	<rdf:type rdf:resource="http://www.w3.org/1999/02/22-rdf-syntax-ns#List"/>
	<rdf:first rdf:nodeID="genid9"/>
</rdf:Description>

<rdf:Description rdf:nodeID="genid9">
	<rdf:type rdf:resource="http://www.w3.org/2002/07/owl#Restriction"/>
	<owl:onProperty rdf:resource="http://www.w3.org/2004/02/skos/core#inScheme"/>
	<owl:hasValue rdf:resource="http://vocab.linkeddata.es/datosabiertos/kos/sector-publico/agenda-municipal/rol"/>
</rdf:Description>

<rdf:Description rdf:nodeID="genid8">
	<rdf:rest rdf:resource="http://www.w3.org/1999/02/22-rdf-syntax-ns#nil"/>
</rdf:Description>

<rdf:Description rdf:nodeID="genid7">
	<rdf:type rdf:resource="http://www.w3.org/2002/07/owl#Class"/>
</rdf:Description>

<rdf:Description rdf:about="http://vocab.linkeddata.es/datosabiertos/def/sector-publico/agenda-municipal##rol">
	<rdfs:comment xml:lang="es">El rol que puede tener un integrante de un evento.</rdfs:comment>
	<rdfs:comment xml:lang="en">The role of a member of an event.</rdfs:comment>
	<rdfs:isDefinedBy>http://vocab.linkeddata.es/datosabiertos/def/sector-publico/agenda-municipal</rdfs:isDefinedBy>
	<rdfs:label xml:lang="es">rol</rdfs:label>
	<rdfs:label xml:lang="en">role</rdfs:label>
</rdf:Description>
<!--  -->
<!-- http://vocab.linkeddata.es/datosabiertos/def/sector-publico/agenda-municipal##rolIntegrante -->

<rdf:Description rdf:about="http://vocab.linkeddata.es/datosabiertos/def/sector-publico/agenda-municipal##rolIntegrante">
	<rdf:type rdf:resource="http://www.w3.org/2002/07/owl#ObjectProperty"/>
	<rdfs:domain rdf:resource="http://vocab.linkeddata.es/datosabiertos/def/sector-publico/agenda-municipal##Evento"/>
	<rdfs:range rdf:resource="http://vocab.linkeddata.es/datosabiertos/def/sector-publico/agenda-municipal##RolIntegranteEvento"/>
	<rdfs:comment xml:lang="es">Rol del integrante de un evento.</rdfs:comment>
	<rdfs:comment xml:lang="en">Role of a  member of an event.</rdfs:comment>
	<rdfs:isDefinedBy xml:lang="es">http://vocab.linkeddata.es/datosabiertos/def/sector-publico/agenda-municipal</rdfs:isDefinedBy>
	<rdfs:label xml:lang="en">member role</rdfs:label>
	<rdfs:label xml:lang="es">rol Integrante</rdfs:label>
</rdf:Description>
<!--  -->
<!-- http://vocab.linkeddata.es/datosabiertos/def/sector-publico/agenda-municipal##tipoAcceso -->

<rdf:Description rdf:about="http://vocab.linkeddata.es/datosabiertos/def/sector-publico/agenda-municipal##tipoAcceso">
	<rdf:type rdf:resource="http://www.w3.org/2002/07/owl#ObjectProperty"/>
	<rdfs:domain rdf:resource="http://vocab.linkeddata.es/datosabiertos/def/sector-publico/agenda-municipal##Evento"/>
	<rdfs:range rdf:nodeID="genid11"/>
</rdf:Description>

<rdf:Description rdf:nodeID="genid11">
	<owl:intersectionOf rdf:nodeID="genid14"/>
</rdf:Description>

<rdf:Description rdf:nodeID="genid14">
	<rdf:type rdf:resource="http://www.w3.org/1999/02/22-rdf-syntax-ns#List"/>
	<rdf:first rdf:resource="http://www.w3.org/2004/02/skos/core#Concept"/>
	<rdf:rest rdf:nodeID="genid12"/>
</rdf:Description>

<rdf:Description rdf:nodeID="genid12">
	<rdf:type rdf:resource="http://www.w3.org/1999/02/22-rdf-syntax-ns#List"/>
	<rdf:first rdf:nodeID="genid13"/>
</rdf:Description>

<rdf:Description rdf:nodeID="genid13">
	<rdf:type rdf:resource="http://www.w3.org/2002/07/owl#Restriction"/>
	<owl:onProperty rdf:resource="http://www.w3.org/2004/02/skos/core#inScheme"/>
	<owl:hasValue rdf:resource="http://vocab.linkeddata.es/datosabiertos/kos/sector-publico/agenda-municipal/tipo-acceso"/>
</rdf:Description>

<rdf:Description rdf:nodeID="genid12">
	<rdf:rest rdf:resource="http://www.w3.org/1999/02/22-rdf-syntax-ns#nil"/>
</rdf:Description>

<rdf:Description rdf:nodeID="genid11">
	<rdf:type rdf:resource="http://www.w3.org/2002/07/owl#Class"/>
</rdf:Description>

<rdf:Description rdf:about="http://vocab.linkeddata.es/datosabiertos/def/sector-publico/agenda-municipal##tipoAcceso">
	<rdfs:comment xml:lang="es">Tipo de asistencia al evento: público, privado o restringido.</rdfs:comment>
	<rdfs:comment xml:lang="en">Type of event attendance: public, private or restricted.</rdfs:comment>
	<rdfs:isDefinedBy>http://vocab.linkeddata.es/datosabiertos/def/sector-publico/agenda-municipal</rdfs:isDefinedBy>
	<rdfs:label xml:lang="en">attendance type</rdfs:label>
	<rdfs:label xml:lang="es">tipo de acceso</rdfs:label>
</rdf:Description>
<!--  -->
<!-- http://vocab.linkeddata.es/datosabiertos/def/sector-publico/agenda-municipal##tipoEvento -->

<rdf:Description rdf:about="http://vocab.linkeddata.es/datosabiertos/def/sector-publico/agenda-municipal##tipoEvento">
	<rdf:type rdf:resource="http://www.w3.org/2002/07/owl#ObjectProperty"/>
	<rdfs:domain rdf:resource="http://vocab.linkeddata.es/datosabiertos/def/sector-publico/agenda-municipal##Evento"/>
	<rdfs:range rdf:nodeID="genid15"/>
</rdf:Description>

<rdf:Description rdf:nodeID="genid15">
	<owl:intersectionOf rdf:nodeID="genid18"/>
</rdf:Description>

<rdf:Description rdf:nodeID="genid18">
	<rdf:type rdf:resource="http://www.w3.org/1999/02/22-rdf-syntax-ns#List"/>
	<rdf:first rdf:resource="http://www.w3.org/2004/02/skos/core#Concept"/>
	<rdf:rest rdf:nodeID="genid16"/>
</rdf:Description>

<rdf:Description rdf:nodeID="genid16">
	<rdf:type rdf:resource="http://www.w3.org/1999/02/22-rdf-syntax-ns#List"/>
	<rdf:first rdf:nodeID="genid17"/>
</rdf:Description>

<rdf:Description rdf:nodeID="genid17">
	<rdf:type rdf:resource="http://www.w3.org/2002/07/owl#Restriction"/>
	<owl:onProperty rdf:resource="http://www.w3.org/2004/02/skos/core#inScheme"/>
	<owl:hasValue rdf:resource="http://vocab.linkeddata.es/datosabiertos/kos/sector-publico/agenda-municipal/tipo-evento"/>
</rdf:Description>

<rdf:Description rdf:nodeID="genid16">
	<rdf:rest rdf:resource="http://www.w3.org/1999/02/22-rdf-syntax-ns#nil"/>
</rdf:Description>

<rdf:Description rdf:nodeID="genid15">
	<rdf:type rdf:resource="http://www.w3.org/2002/07/owl#Class"/>
</rdf:Description>

<rdf:Description rdf:about="http://vocab.linkeddata.es/datosabiertos/def/sector-publico/agenda-municipal##tipoEvento">
	<rdfs:comment xml:lang="es">Tipología que define a qué categoría pertenece el evento. Los tipos de evento se representan mediante una lista de conceptos.</rdfs:comment>
	<rdfs:comment xml:lang="en">Typology that defines to what category the event belongs. Event types are represented by a list of concepts.</rdfs:comment>
	<rdfs:isDefinedBy>http://vocab.linkeddata.es/datosabiertos/def/sector-publico/agenda-municipal</rdfs:isDefinedBy>
	<rdfs:label xml:lang="es">event type</rdfs:label>
	<rdfs:label>tipo de evento</rdfs:label>
</rdf:Description>
<!--  -->
<!-- http://vocab.linkeddata.es/datosabiertos/def/sector-publico/agenda-municipal##tipoSesion -->

<rdf:Description rdf:about="http://vocab.linkeddata.es/datosabiertos/def/sector-publico/agenda-municipal##tipoSesion">
	<rdf:type rdf:resource="http://www.w3.org/2002/07/owl#ObjectProperty"/>
	<rdfs:domain rdf:resource="http://vocab.linkeddata.es/datosabiertos/def/sector-publico/agenda-municipal##Evento"/>
	<rdfs:range rdf:nodeID="genid19"/>
</rdf:Description>

<rdf:Description rdf:nodeID="genid19">
	<owl:intersectionOf rdf:nodeID="genid22"/>
</rdf:Description>

<rdf:Description rdf:nodeID="genid22">
	<rdf:type rdf:resource="http://www.w3.org/1999/02/22-rdf-syntax-ns#List"/>
	<rdf:first rdf:resource="http://www.w3.org/2004/02/skos/core#Concept"/>
	<rdf:rest rdf:nodeID="genid20"/>
</rdf:Description>

<rdf:Description rdf:nodeID="genid20">
	<rdf:type rdf:resource="http://www.w3.org/1999/02/22-rdf-syntax-ns#List"/>
	<rdf:first rdf:nodeID="genid21"/>
</rdf:Description>

<rdf:Description rdf:nodeID="genid21">
	<rdf:type rdf:resource="http://www.w3.org/2002/07/owl#Restriction"/>
	<owl:onProperty rdf:resource="http://www.w3.org/2004/02/skos/core#inScheme"/>
	<owl:hasValue rdf:resource="http://vocab.linkeddata.es/datosabiertos/kos/sector-publico/agenda-municipal/tipo-sesion"/>
</rdf:Description>

<rdf:Description rdf:nodeID="genid20">
	<rdf:rest rdf:resource="http://www.w3.org/1999/02/22-rdf-syntax-ns#nil"/>
</rdf:Description>

<rdf:Description rdf:nodeID="genid19">
	<rdf:type rdf:resource="http://www.w3.org/2002/07/owl#Class"/>
</rdf:Description>

<rdf:Description rdf:about="http://vocab.linkeddata.es/datosabiertos/def/sector-publico/agenda-municipal##tipoSesion">
	<rdfs:comment xml:lang="en">For the events of collegiate bodies, the type id session defines if the session is ordinary, extraordinary or extraordinary urgent</rdfs:comment>
	<rdfs:comment xml:lang="es">Para los eventos de órganos colegiados, tipo de sesión puede ser ordinaria, extraordinaria o extraordinaria urgente</rdfs:comment>
	<rdfs:isDefinedBy>http://vocab.linkeddata.es/datosabiertos/def/sector-publico/agenda-municipal</rdfs:isDefinedBy>
	<rdfs:label xml:lang="en">session type</rdfs:label>
	<rdfs:label xml:lang="es">tipo de sesion</rdfs:label>
</rdf:Description>
<!--  -->
<!-- http://vocab.linkeddata.es/datosabiertos/def/sector-publico/organizacion#ambitoCompetencias -->

<rdf:Description rdf:about="http://vocab.linkeddata.es/datosabiertos/def/sector-publico/organizacion#ambitoCompetencias">
	<rdf:type rdf:resource="http://www.w3.org/2002/07/owl#ObjectProperty"/>
	<rdfs:domain rdf:resource="http://www.w3.org/ns/org#Organization"/>
	<rdfs:range rdf:resource="http://dbpedia.org/ontology/GovernmentalAdministrativeRegion"/>
	<rdfs:comment xml:lang="en">Competence Scope</rdfs:comment>
	<rdfs:comment>Ámbito territorial de ejercicio de competencias de una organización.</rdfs:comment>
	<rdfs:isDefinedBy>http://vocab.linkeddata.es/datosabiertos/def/sector-publico/organizacion#</rdfs:isDefinedBy>
	<rdfs:label>Ámbito de Competencias</rdfs:label>
</rdf:Description>
<!--  -->
<!-- http://www.w3.org/2004/02/skos/core#inScheme -->

<rdf:Description rdf:about="http://www.w3.org/2004/02/skos/core#inScheme">
	<rdf:type rdf:resource="http://www.w3.org/2002/07/owl#ObjectProperty"/>
	<rdfs:range rdf:resource="http://www.w3.org/2004/02/skos/core#ConceptScheme"/>
	<rdfs:isDefinedBy xml:lang="en">http://www.w3.org/2004/02/skos/core</rdfs:isDefinedBy>
	<rdfs:label xml:lang="en">is in scheme</rdfs:label>
	<skos:definition xml:lang="en">Relates a resource (for example a concept) to a concept scheme in which it is included.</skos:definition>
	<skos:scopeNote xml:lang="en">A concept may be a member of more than one concept scheme.</skos:scopeNote>
</rdf:Description>
<!--  -->
<!-- http://www.w3.org/ns/org#hasMembership -->

<rdf:Description rdf:about="http://www.w3.org/ns/org#hasMembership">
	<rdf:type rdf:resource="http://www.w3.org/2002/07/owl#ObjectProperty"/>
	<owl:inverseOf rdf:resource="http://www.w3.org/ns/org#member"/>
	<rdfs:domain rdf:resource="http://xmlns.com/foaf/0.1/Agent"/>
	<rdfs:range rdf:resource="http://www.w3.org/ns/org#Membership"/>
	<rdfs:comment xml:lang="it">Indica una relazione di appartenenza che coinvolge un Agent. È l'inverso di `org:member`.</rdfs:comment>
	<rdfs:comment xml:lang="en">Indicates a membership relationship that the Agent plays. Inverse of `org:member`.</rdfs:comment>
	<rdfs:comment xml:lang="fr">Indique pour cet Agent un engagement dans une Organisation. Inverse de `org:member`.</rdfs:comment>
	<rdfs:comment xml:lang="es">Relación de pertenencia o afiliación a una organización en la que el agente desempeña un cargo o función. Es la relación inversa de `org:member`.</rdfs:comment>
	<rdfs:comment xml:lang="ja">エージェントが担う構成員関係を示します。</rdfs:comment>
	<rdfs:isDefinedBy rdf:resource="http://www.w3.org/ns/org"/>
	<rdfs:label xml:lang="it">appartenenza</rdfs:label>
	<rdfs:label xml:lang="fr">engagement</rdfs:label>
	<rdfs:label xml:lang="en">membership</rdfs:label>
	<rdfs:label xml:lang="es">tiene membresía</rdfs:label>
</rdf:Description>
<!--  -->
<!-- http://www.w3.org/ns/org#member -->

<rdf:Description rdf:about="http://www.w3.org/ns/org#member">
	<rdf:type rdf:resource="http://www.w3.org/2002/07/owl#ObjectProperty"/>
	<rdf:type rdf:resource="http://www.w3.org/2002/07/owl#FunctionalProperty"/>
	<rdfs:domain rdf:resource="http://www.w3.org/ns/org#Membership"/>
	<rdfs:range rdf:resource="http://xmlns.com/foaf/0.1/Agent"/>
	<rdfs:comment xml:lang="it">Indica la Person (o un altro Agent) coinvolto in una relazione di Membership. È l'inverso di `org:hasMembership`.</rdfs:comment>
	<rdfs:comment xml:lang="en">Indicates the Person (or other Agent including Organization) involved in the Membership relationship. Inverse of `org:hasMembership`</rdfs:comment>
	<rdfs:comment xml:lang="fr">Indique une personne (ou tout autre Agent, y compris une Organisation) impliqué dans la relation d'Engagement. Inverse de `org:hasMembership`</rdfs:comment>
	<rdfs:comment xml:lang="es">Persona (u otro agente, incluyendo una organización) que participa en la relación de membresía. Es la relación inversa de `org:hasMembership`.</rdfs:comment>
	<rdfs:comment xml:lang="ja">構成員関係に含まれている人（または、組織を含んでいる他のエージェント）を示します。</rdfs:comment>
	<rdfs:isDefinedBy rdf:resource="http://www.w3.org/ns/org"/>
	<rdfs:label xml:lang="es">es condición de miembro sobre agente</rdfs:label>
	<rdfs:label xml:lang="en">member</rdfs:label>
	<rdfs:label xml:lang="fr">membre</rdfs:label>
	<rdfs:label xml:lang="it">membro</rdfs:label>
</rdf:Description>
<!--  -->
<!-- http://www.w3.org/ns/org#organization -->

<rdf:Description rdf:about="http://www.w3.org/ns/org#organization">
	<rdf:type rdf:resource="http://www.w3.org/2002/07/owl#ObjectProperty"/>
	<rdf:type rdf:resource="http://www.w3.org/2002/07/owl#FunctionalProperty"/>
	<rdfs:domain rdf:resource="http://www.w3.org/ns/org#Membership"/>
	<rdfs:range rdf:resource="http://www.w3.org/ns/org#Organization"/>
	<rdfs:comment xml:lang="it">Indica l'Organization in cui l'Agent è un membro.</rdfs:comment>
	<rdfs:comment xml:lang="en">Indicates Organization in which the Agent is a member.</rdfs:comment>
	<rdfs:comment xml:lang="fr">Indique l'Organization dont l'agent est membre.</rdfs:comment>
	<rdfs:comment xml:lang="es">Organización a la que pertenece el agente en calidad de miembro.</rdfs:comment>
	<rdfs:comment xml:lang="ja">エージェントがメンバーである組織を示します。</rdfs:comment>
	<rdfs:isDefinedBy rdf:resource="http://www.w3.org/ns/org"/>
	<rdfs:label xml:lang="es">es condición de miembro sobre organización</rdfs:label>
	<rdfs:label xml:lang="fr">organisation</rdfs:label>
	<rdfs:label xml:lang="en">organization</rdfs:label>
	<rdfs:label xml:lang="it">organizzazione</rdfs:label>
</rdf:Description>
<!--  -->
<!-- http://www.w3.org/ns/org#role -->

<rdf:Description rdf:about="http://www.w3.org/ns/org#role">
	<rdf:type rdf:resource="http://www.w3.org/2002/07/owl#ObjectProperty"/>
	<rdfs:domain rdf:resource="http://www.w3.org/ns/org#Membership"/>
	<rdfs:range rdf:resource="http://www.w3.org/ns/org#Role"/>
	<rdfs:comment xml:lang="es">Actividad que el agente desempeña en una relación de pertenencia a una organización.</rdfs:comment>
	<rdfs:comment xml:lang="it">Indica il Role che un Agent ricopre in una relazione di Membership con una Organization</rdfs:comment>
	<rdfs:comment xml:lang="en">Indicates the Role that the Agent plays in a Membership relationship with an Organization.</rdfs:comment>
	<rdfs:comment xml:lang="fr">Indique le Rôle de l'Agent dans son Engagement avec l'Organisation.</rdfs:comment>
	<rdfs:comment xml:lang="ja">エージェントが組織との構成員関係において担う役割を示します。ポストの保持者が担う役割を示すためにorg:Postで用いることもできます。</rdfs:comment>
	<rdfs:isDefinedBy rdf:resource="http://www.w3.org/ns/org"/>
	<rdfs:label xml:lang="es">desempeña la actividad de</rdfs:label>
	<rdfs:label xml:lang="en">role</rdfs:label>
	<rdfs:label xml:lang="it">ruolo</rdfs:label>
	<rdfs:label xml:lang="fr">rôle</rdfs:label>
</rdf:Description>
<!--  -->
<!-- rdfs:label -->

<rdf:Description rdf:about="rdfs:label">
	<rdf:type rdf:resource="http://www.w3.org/2002/07/owl#ObjectProperty"/>
</rdf:Description>
<!--  -->
<!--  -->
<!--  -->
<!-- ################################################################# -->
<!-- # -->
<!-- #    Data properties -->
<!-- # -->
<!-- ################################################################# -->
<!--  -->
<!--  -->
<!-- http://schema.org/address -->

<rdf:Description rdf:about="http://schema.org/address">
	<rdf:type rdf:resource="http://www.w3.org/2002/07/owl#DatatypeProperty"/>
	<rdfs:domain rdf:resource="http://schema.org/Place"/>
	<rdfs:range rdf:resource="http://www.w3.org/2001/XMLSchema#string"/>
	<rdfs:comment xml:lang="en">Physical address of the item.</rdfs:comment>
	<rdfs:isDefinedBy rdf:resource="https://schema.org/address"/>
	<rdfs:label xml:lang="en">address</rdfs:label>
</rdf:Description>
<!--  -->
<!-- http://schema.org/description -->

<rdf:Description rdf:about="http://schema.org/description">
	<rdf:type rdf:resource="http://www.w3.org/2002/07/owl#DatatypeProperty"/>
	<rdfs:domain rdf:resource="http://www.w3.org/2002/07/owl#Thing"/>
	<rdfs:range rdf:resource="http://www.w3.org/2001/XMLSchema#string"/>
	<rdfs:comment xml:lang="en">A description of the item.</rdfs:comment>
	<rdfs:isDefinedBy rdf:resource="https://schema.org/description"/>
	<rdfs:label xml:lang="en">description</rdfs:label>
</rdf:Description>
<!--  -->
<!-- http://schema.org/endDate -->

<rdf:Description rdf:about="http://schema.org/endDate">
	<rdf:type rdf:resource="http://www.w3.org/2002/07/owl#DatatypeProperty"/>
	<rdfs:domain rdf:resource="http://schema.org/Event"/>
	<rdfs:range rdf:resource="http://www.w3.org/2001/XMLSchema#dateTime"/>
	<rdfs:comment xml:lang="en">The end date and time of the item (in &lt;a href="http://en.wikipedia.org/wiki/ISO_8601"&gt;ISO 8601 date format&lt;/a&gt;).</rdfs:comment>
	<rdfs:isDefinedBy rdf:resource="https://schema.org/endDate"/>
	<rdfs:label xml:lang="en">endDate</rdfs:label>
</rdf:Description>
<!--  -->
<!-- http://schema.org/startDate -->

<rdf:Description rdf:about="http://schema.org/startDate">
	<rdf:type rdf:resource="http://www.w3.org/2002/07/owl#DatatypeProperty"/>
	<rdfs:domain rdf:resource="http://schema.org/Event"/>
	<rdfs:range rdf:resource="http://www.w3.org/2001/XMLSchema#dateTime"/>
	<rdfs:comment xml:lang="en">The start date and time of the item (in &lt;a href="http://en.wikipedia.org/wiki/ISO_8601"&gt;ISO 8601 date format&lt;/a&gt;).</rdfs:comment>
	<rdfs:isDefinedBy rdf:resource="https://schema.org/startDate"/>
	<rdfs:label xml:lang="en">startDate</rdfs:label>
</rdf:Description>
<!--  -->
<!-- http://schema.org/url -->

<rdf:Description rdf:about="http://schema.org/url">
	<rdf:type rdf:resource="http://www.w3.org/2002/07/owl#DatatypeProperty"/>
	<rdfs:domain rdf:resource="http://www.w3.org/2002/07/owl#Thing"/>
	<rdfs:range rdf:resource="http://www.w3.org/2001/XMLSchema#anyURI"/>
	<rdfs:comment xml:lang="en">url of the item.</rdfs:comment>
	<rdfs:isDefinedBy rdf:resource="https://schema.org/url"/>
	<rdfs:label xml:lang="en">url</rdfs:label>
</rdf:Description>
<!--  -->
<!-- http://vocab.linkeddata.es/datosabiertos/def/sector-publico/agenda-municipal##formato -->

<rdf:Description rdf:about="http://vocab.linkeddata.es/datosabiertos/def/sector-publico/agenda-municipal##formato">
	<rdf:type rdf:resource="http://www.w3.org/2002/07/owl#DatatypeProperty"/>
	<rdfs:domain rdf:resource="http://vocab.linkeddata.es/datosabiertos/def/sector-publico/agenda-municipal##Documentacion"/>
	<rdfs:range rdf:nodeID="genid23"/>
</rdf:Description>

<rdf:Description rdf:nodeID="genid23">
	<rdf:type rdf:resource="http://www.w3.org/2000/01/rdf-schema#Datatype"/>
	<owl:oneOf rdf:nodeID="genid26"/>
</rdf:Description>

<rdf:Description rdf:nodeID="genid26">
	<rdf:type rdf:resource="http://www.w3.org/1999/02/22-rdf-syntax-ns#List"/>
	<rdf:first>imagen</rdf:first>
	<rdf:rest rdf:nodeID="genid25"/>
</rdf:Description>

<rdf:Description rdf:nodeID="genid25">
	<rdf:type rdf:resource="http://www.w3.org/1999/02/22-rdf-syntax-ns#List"/>
	<rdf:first>texto</rdf:first>
	<rdf:rest rdf:nodeID="genid24"/>
</rdf:Description>

<rdf:Description rdf:nodeID="genid24">
	<rdf:type rdf:resource="http://www.w3.org/1999/02/22-rdf-syntax-ns#List"/>
	<rdf:first>video</rdf:first>
	<rdf:rest rdf:resource="http://www.w3.org/1999/02/22-rdf-syntax-ns#nil"/>
</rdf:Description>

<rdf:Description rdf:about="http://vocab.linkeddata.es/datosabiertos/def/sector-publico/agenda-municipal##formato">
	<rdfs:comment xml:lang="en">Format of the document: image, video, text.</rdfs:comment>
	<rdfs:comment xml:lang="es">Formato del documento: imagen, video, texto.</rdfs:comment>
	<rdfs:isDefinedBy xml:lang="es">http://vocab.linkeddata.es/datosabiertos/def/sector-publico/agenda-municipal</rdfs:isDefinedBy>
	<rdfs:label xml:lang="en">format</rdfs:label>
	<rdfs:label xml:lang="es">formato</rdfs:label>
</rdf:Description>
<!--  -->
<!-- http://vocab.linkeddata.es/datosabiertos/def/sector-publico/agenda-municipal##nombreDoc -->

<rdf:Description rdf:about="http://vocab.linkeddata.es/datosabiertos/def/sector-publico/agenda-municipal##nombreDoc">
	<rdf:type rdf:resource="http://www.w3.org/2002/07/owl#DatatypeProperty"/>
	<rdfs:domain rdf:resource="http://vocab.linkeddata.es/datosabiertos/def/sector-publico/agenda-municipal##Documentacion"/>
	<rdfs:range rdf:resource="http://www.w3.org/2001/XMLSchema#string"/>
	<rdfs:comment xml:lang="en">Name of the documentation such as minutes of meeting, motion, etc.</rdfs:comment>
	<rdfs:comment xml:lang="es">Nombre de la documentación tal como acta de reunión, moción, etc.</rdfs:comment>
	<rdfs:isDefinedBy>http://vocab.linkeddata.es/datosabiertos/def/sector-publico/agenda-municipal</rdfs:isDefinedBy>
	<rdfs:label xml:lang="en">documentation name</rdfs:label>
	<rdfs:label xml:lang="es">nombre documentación</rdfs:label>
</rdf:Description>
<!--  -->
<!-- http://vocab.linkeddata.es/datosabiertos/def/sector-publico/agenda-municipal##publico -->

<rdf:Description rdf:about="http://vocab.linkeddata.es/datosabiertos/def/sector-publico/agenda-municipal##publico">
	<rdf:type rdf:resource="http://www.w3.org/2002/07/owl#DatatypeProperty"/>
	<rdf:type rdf:resource="http://www.w3.org/2002/07/owl#FunctionalProperty"/>
	<rdfs:domain rdf:resource="http://vocab.linkeddata.es/datosabiertos/def/sector-publico/agenda-municipal##Documentacion"/>
	<rdfs:range rdf:resource="http://www.w3.org/2001/XMLSchema#boolean"/>
	<rdfs:comment xml:lang="es">Si la documentación es de acceso público o no (privado).</rdfs:comment>
	<rdfs:comment xml:lang="en">Whether the documentation is public access or not (private).</rdfs:comment>
	<rdfs:isDefinedBy>http://vocab.linkeddata.es/datosabiertos/def/sector-publico/agenda-municipal</rdfs:isDefinedBy>
	<rdfs:label xml:lang="en">public</rdfs:label>
	<rdfs:label xml:lang="es">público</rdfs:label>
</rdf:Description>
<!--  -->
<!-- http://vocab.linkeddata.es/datosabiertos/def/sector-publico/agenda-municipal##uriDoc -->

<rdf:Description rdf:about="http://vocab.linkeddata.es/datosabiertos/def/sector-publico/agenda-municipal##uriDoc">
	<rdf:type rdf:resource="http://www.w3.org/2002/07/owl#DatatypeProperty"/>
	<rdf:type rdf:resource="http://www.w3.org/2002/07/owl#FunctionalProperty"/>
	<rdfs:domain rdf:resource="http://vocab.linkeddata.es/datosabiertos/def/sector-publico/agenda-municipal##Documentacion"/>
	<rdfs:range rdf:resource="http://www.w3.org/2001/XMLSchema#anyURI"/>
	<rdfs:comment xml:lang="es">URI donde se encuentra la documentación.</rdfs:comment>
	<rdfs:comment xml:lang="en">URI where the documentation is located.</rdfs:comment>
	<rdfs:isDefinedBy>http://vocab.linkeddata.es/datosabiertos/def/sector-publico/agenda-municipal</rdfs:isDefinedBy>
	<rdfs:label xml:lang="es">uri documentación</rdfs:label>
	<rdfs:label xml:lang="en">uri documentation</rdfs:label>
</rdf:Description>
<!--  -->
<!-- http://xmlns.com/foaf/0.1/name -->

<rdf:Description rdf:about="http://xmlns.com/foaf/0.1/name">
	<rdf:type rdf:resource="http://www.w3.org/2002/07/owl#DatatypeProperty"/>
	<rdfs:domain rdf:resource="http://www.w3.org/2002/07/owl#Thing"/>
	<rdfs:range rdf:resource="http://www.w3.org/2000/01/rdf-schema#Literal"/>
	<rdfs:comment xml:lang="en">A name for some thing.</rdfs:comment>
	<rdfs:isDefinedBy xml:lang="en">http://xmlns.com/foaf/0.1/</rdfs:isDefinedBy>
	<rdfs:label xml:lang="en">name</rdfs:label>
</rdf:Description>
<!--  -->
<!--  -->
<!--  -->
<!-- ################################################################# -->
<!-- # -->
<!-- #    Classes -->
<!-- # -->
<!-- ################################################################# -->
<!--  -->
<!--  -->
<!-- http://dbpedia.org/ontology/District -->

<rdf:Description rdf:about="http://dbpedia.org/ontology/District">
	<rdf:type rdf:resource="http://www.w3.org/2002/07/owl#Class"/>
	<rdfs:subClassOf rdf:resource="http://dbpedia.org/ontology/GovernmentalAdministrativeRegion"/>
	<rdfs:isDefinedBy xml:lang="en">http://mappings.dbpedia.org/index.php/OntologyClass:District</rdfs:isDefinedBy>
	<rdfs:label xml:lang="en">district</rdfs:label>
</rdf:Description>
<!--  -->
<!-- http://dbpedia.org/ontology/GovernmentalAdministrativeRegion -->

<rdf:Description rdf:about="http://dbpedia.org/ontology/GovernmentalAdministrativeRegion">
	<rdf:type rdf:resource="http://www.w3.org/2002/07/owl#Class"/>
	<rdfs:comment xml:lang="en">An administrative body governing some territorial unity, in this case a governmental administrative body</rdfs:comment>
	<rdfs:label xml:lang="en">governmental administrative region</rdfs:label>
</rdf:Description>
<!--  -->
<!-- http://dbpedia.org/ontology/Municipality -->

<rdf:Description rdf:about="http://dbpedia.org/ontology/Municipality">
	<rdf:type rdf:resource="http://www.w3.org/2002/07/owl#Class"/>
	<rdfs:subClassOf rdf:resource="http://dbpedia.org/ontology/GovernmentalAdministrativeRegion"/>
	<rdfs:comment xml:lang="es">Un Municipio es el ente local definido en el artículo 140 de la Constitución española y la entidad básica de la organización territorial del Estado según el artículo 1 de la Ley 7/1985, de 2 de abril, Reguladora de las Bases del Régimen Local. Tiene personalidad jurídica y plena capacidad para el cumplimiento de sus fines. La delimitación territorial de Municipio está recogida del REgistro Central de Cartografía del IGN.</rdfs:comment>
	<rdfs:isDefinedBy>http://dbpedia.org/ontology/</rdfs:isDefinedBy>
	<rdfs:label xml:lang="en">municipality</rdfs:label>
</rdf:Description>
<!--  -->
<!-- http://schema.org/Event -->

<rdf:Description rdf:about="http://schema.org/Event">
	<rdf:type rdf:resource="http://www.w3.org/2002/07/owl#Class"/>
	<rdfs:comment>An event happening at a certain time and location, such as a concert, lecture, or festival. Ticketing information may be added via the offers property. Repeated events may be structured as separate Event objects.</rdfs:comment>
	<rdfs:isDefinedBy>https://schema.org/Event</rdfs:isDefinedBy>
	<rdfs:label xml:lang="en">Event</rdfs:label>
</rdf:Description>
<!--  -->
<!-- http://schema.org/Place -->

<rdf:Description rdf:about="http://schema.org/Place">
	<rdf:type rdf:resource="http://www.w3.org/2002/07/owl#Class"/>
	<rdfs:comment>Entities that have a somewhat fixed, physical extension.</rdfs:comment>
	<rdfs:isDefinedBy>https://schema.org/Event</rdfs:isDefinedBy>
	<rdfs:label>Place</rdfs:label>
</rdf:Description>
<!--  -->
<!-- http://schema.org/Text -->

<rdf:Description rdf:about="http://schema.org/Text">
	<rdf:type rdf:resource="http://www.w3.org/2002/07/owl#Class"/>
	<rdfs:comment xml:lang="en">Data type: Text.</rdfs:comment>
	<rdfs:label xml:lang="en">Text</rdfs:label>
</rdf:Description>
<!--  -->
<!-- http://schema.org/Thing -->

<rdf:Description rdf:about="http://schema.org/Thing">
	<rdf:type rdf:resource="http://www.w3.org/2002/07/owl#Class"/>
	<rdfs:comment xml:lang="en">The most generic type of item.</rdfs:comment>
	<rdfs:isDefinedBy>https://schema.org/Thing</rdfs:isDefinedBy>
	<rdfs:label xml:lang="en">Thing</rdfs:label>
</rdf:Description>
<!--  -->
<!-- http://vocab.linkeddata.es/datosabiertos/def/sector-publico/agenda-municipal##Documentacion -->

<rdf:Description rdf:about="http://vocab.linkeddata.es/datosabiertos/def/sector-publico/agenda-municipal##Documentacion">
	<rdf:type rdf:resource="http://www.w3.org/2002/07/owl#Class"/>
	<rdfs:comment xml:lang="en">Reference to the documentation associated with the event.</rdfs:comment>
	<rdfs:comment xml:lang="es">Referencia a la documentación asociada al evento.</rdfs:comment>
	<rdfs:isDefinedBy>http://vocab.linkeddata.es/datosabiertos/def/sector-publico/agenda-municipal</rdfs:isDefinedBy>
	<rdfs:label xml:lang="es">Documentación</rdfs:label>
	<rdfs:label xml:lang="en">Documentation</rdfs:label>
</rdf:Description>
<!--  -->
<!-- http://vocab.linkeddata.es/datosabiertos/def/sector-publico/agenda-municipal##Evento -->

<rdf:Description rdf:about="http://vocab.linkeddata.es/datosabiertos/def/sector-publico/agenda-municipal##Evento">
	<rdf:type rdf:resource="http://www.w3.org/2002/07/owl#Class"/>
	<rdfs:subClassOf rdf:resource="http://schema.org/Event"/>
	<rdfs:subClassOf rdf:nodeID="genid27"/>
</rdf:Description>

<rdf:Description rdf:nodeID="genid27">
	<owl:intersectionOf rdf:nodeID="genid30"/>
</rdf:Description>

<rdf:Description rdf:nodeID="genid30">
	<rdf:type rdf:resource="http://www.w3.org/1999/02/22-rdf-syntax-ns#List"/>
	<rdf:first rdf:nodeID="genid31"/>
</rdf:Description>

<rdf:Description rdf:nodeID="genid31">
	<rdf:type rdf:resource="http://www.w3.org/2002/07/owl#Restriction"/>
	<owl:onProperty rdf:resource="http://vocab.linkeddata.es/datosabiertos/def/sector-publico/agenda-municipal##canal"/>
	<owl:allValuesFrom rdf:resource="http://www.w3.org/2004/02/skos/core#Concept"/>
</rdf:Description>

<rdf:Description rdf:nodeID="genid30">
	<rdf:rest rdf:nodeID="genid28"/>
</rdf:Description>

<rdf:Description rdf:nodeID="genid28">
	<rdf:type rdf:resource="http://www.w3.org/1999/02/22-rdf-syntax-ns#List"/>
	<rdf:first rdf:nodeID="genid29"/>
</rdf:Description>

<rdf:Description rdf:nodeID="genid29">
	<rdf:type rdf:resource="http://www.w3.org/2002/07/owl#Restriction"/>
	<owl:onProperty rdf:resource="http://vocab.linkeddata.es/datosabiertos/def/sector-publico/agenda-municipal##canal"/>
	<owl:maxQualifiedCardinality rdf:datatype="http://www.w3.org/2001/XMLSchema#nonNegativeInteger">1</owl:maxQualifiedCardinality>
	<owl:onClass rdf:resource="http://www.w3.org/2004/02/skos/core#Concept"/>
</rdf:Description>

<rdf:Description rdf:nodeID="genid28">
	<rdf:rest rdf:resource="http://www.w3.org/1999/02/22-rdf-syntax-ns#nil"/>
</rdf:Description>

<rdf:Description rdf:nodeID="genid27">
	<rdf:type rdf:resource="http://www.w3.org/2002/07/owl#Class"/>
</rdf:Description>

<rdf:Description rdf:about="http://vocab.linkeddata.es/datosabiertos/def/sector-publico/agenda-municipal##Evento">
	<rdfs:subClassOf rdf:nodeID="genid32"/>
</rdf:Description>

<rdf:Description rdf:nodeID="genid32">
	<owl:intersectionOf rdf:nodeID="genid35"/>
</rdf:Description>

<rdf:Description rdf:nodeID="genid35">
	<rdf:type rdf:resource="http://www.w3.org/1999/02/22-rdf-syntax-ns#List"/>
	<rdf:first rdf:nodeID="genid36"/>
</rdf:Description>

<rdf:Description rdf:nodeID="genid36">
	<rdf:type rdf:resource="http://www.w3.org/2002/07/owl#Restriction"/>
	<owl:onProperty rdf:resource="http://vocab.linkeddata.es/datosabiertos/def/sector-publico/agenda-municipal##rolIntegrante"/>
	<owl:allValuesFrom rdf:resource="http://vocab.linkeddata.es/datosabiertos/def/sector-publico/agenda-municipal##RolIntegranteEvento"/>
</rdf:Description>

<rdf:Description rdf:nodeID="genid35">
	<rdf:rest rdf:nodeID="genid33"/>
</rdf:Description>

<rdf:Description rdf:nodeID="genid33">
	<rdf:type rdf:resource="http://www.w3.org/1999/02/22-rdf-syntax-ns#List"/>
	<rdf:first rdf:nodeID="genid34"/>
</rdf:Description>

<rdf:Description rdf:nodeID="genid34">
	<rdf:type rdf:resource="http://www.w3.org/2002/07/owl#Restriction"/>
	<owl:onProperty rdf:resource="http://vocab.linkeddata.es/datosabiertos/def/sector-publico/agenda-municipal##rolIntegrante"/>
	<owl:qualifiedCardinality rdf:datatype="http://www.w3.org/2001/XMLSchema#nonNegativeInteger">1</owl:qualifiedCardinality>
	<owl:onClass rdf:resource="http://vocab.linkeddata.es/datosabiertos/def/sector-publico/agenda-municipal##RolIntegranteEvento"/>
</rdf:Description>

<rdf:Description rdf:nodeID="genid33">
	<rdf:rest rdf:resource="http://www.w3.org/1999/02/22-rdf-syntax-ns#nil"/>
</rdf:Description>

<rdf:Description rdf:nodeID="genid32">
	<rdf:type rdf:resource="http://www.w3.org/2002/07/owl#Class"/>
</rdf:Description>

<rdf:Description rdf:about="http://vocab.linkeddata.es/datosabiertos/def/sector-publico/agenda-municipal##Evento">
	<rdfs:subClassOf rdf:nodeID="genid37"/>
</rdf:Description>

<rdf:Description rdf:nodeID="genid37">
	<owl:intersectionOf rdf:nodeID="genid40"/>
</rdf:Description>

<rdf:Description rdf:nodeID="genid40">
	<rdf:type rdf:resource="http://www.w3.org/1999/02/22-rdf-syntax-ns#List"/>
	<rdf:first rdf:nodeID="genid41"/>
</rdf:Description>

<rdf:Description rdf:nodeID="genid41">
	<rdf:type rdf:resource="http://www.w3.org/2002/07/owl#Restriction"/>
	<owl:onProperty rdf:resource="http://vocab.linkeddata.es/datosabiertos/def/sector-publico/agenda-municipal##tipoAcceso"/>
	<owl:allValuesFrom rdf:resource="http://www.w3.org/2004/02/skos/core#Concept"/>
</rdf:Description>

<rdf:Description rdf:nodeID="genid40">
	<rdf:rest rdf:nodeID="genid38"/>
</rdf:Description>

<rdf:Description rdf:nodeID="genid38">
	<rdf:type rdf:resource="http://www.w3.org/1999/02/22-rdf-syntax-ns#List"/>
	<rdf:first rdf:nodeID="genid39"/>
</rdf:Description>

<rdf:Description rdf:nodeID="genid39">
	<rdf:type rdf:resource="http://www.w3.org/2002/07/owl#Restriction"/>
	<owl:onProperty rdf:resource="http://vocab.linkeddata.es/datosabiertos/def/sector-publico/agenda-municipal##tipoAcceso"/>
	<owl:maxQualifiedCardinality rdf:datatype="http://www.w3.org/2001/XMLSchema#nonNegativeInteger">1</owl:maxQualifiedCardinality>
	<owl:onClass rdf:resource="http://www.w3.org/2004/02/skos/core#Concept"/>
</rdf:Description>

<rdf:Description rdf:nodeID="genid38">
	<rdf:rest rdf:resource="http://www.w3.org/1999/02/22-rdf-syntax-ns#nil"/>
</rdf:Description>

<rdf:Description rdf:nodeID="genid37">
	<rdf:type rdf:resource="http://www.w3.org/2002/07/owl#Class"/>
</rdf:Description>

<rdf:Description rdf:about="http://vocab.linkeddata.es/datosabiertos/def/sector-publico/agenda-municipal##Evento">
	<rdfs:subClassOf rdf:nodeID="genid42"/>
</rdf:Description>

<rdf:Description rdf:nodeID="genid42">
	<owl:intersectionOf rdf:nodeID="genid45"/>
</rdf:Description>

<rdf:Description rdf:nodeID="genid45">
	<rdf:type rdf:resource="http://www.w3.org/1999/02/22-rdf-syntax-ns#List"/>
	<rdf:first rdf:nodeID="genid46"/>
</rdf:Description>

<rdf:Description rdf:nodeID="genid46">
	<rdf:type rdf:resource="http://www.w3.org/2002/07/owl#Restriction"/>
	<owl:onProperty rdf:resource="http://vocab.linkeddata.es/datosabiertos/def/sector-publico/agenda-municipal##tipoSesion"/>
	<owl:allValuesFrom rdf:resource="http://www.w3.org/2004/02/skos/core#Concept"/>
</rdf:Description>

<rdf:Description rdf:nodeID="genid45">
	<rdf:rest rdf:nodeID="genid43"/>
</rdf:Description>

<rdf:Description rdf:nodeID="genid43">
	<rdf:type rdf:resource="http://www.w3.org/1999/02/22-rdf-syntax-ns#List"/>
	<rdf:first rdf:nodeID="genid44"/>
</rdf:Description>

<rdf:Description rdf:nodeID="genid44">
	<rdf:type rdf:resource="http://www.w3.org/2002/07/owl#Restriction"/>
	<owl:onProperty rdf:resource="http://vocab.linkeddata.es/datosabiertos/def/sector-publico/agenda-municipal##tipoSesion"/>
	<owl:maxQualifiedCardinality rdf:datatype="http://www.w3.org/2001/XMLSchema#nonNegativeInteger">1</owl:maxQualifiedCardinality>
	<owl:onClass rdf:resource="http://www.w3.org/2004/02/skos/core#Concept"/>
</rdf:Description>

<rdf:Description rdf:nodeID="genid43">
	<rdf:rest rdf:resource="http://www.w3.org/1999/02/22-rdf-syntax-ns#nil"/>
</rdf:Description>

<rdf:Description rdf:nodeID="genid42">
	<rdf:type rdf:resource="http://www.w3.org/2002/07/owl#Class"/>
</rdf:Description>

<rdf:Description rdf:about="http://vocab.linkeddata.es/datosabiertos/def/sector-publico/agenda-municipal##Evento">
	<rdfs:subClassOf rdf:nodeID="genid47"/>
</rdf:Description>

<rdf:Description rdf:nodeID="genid47">
	<rdf:type rdf:resource="http://www.w3.org/2002/07/owl#Restriction"/>
	<owl:onProperty rdf:resource="http://vocab.linkeddata.es/datosabiertos/def/sector-publico/agenda-municipal##documentacion"/>
	<owl:allValuesFrom rdf:resource="http://vocab.linkeddata.es/datosabiertos/def/sector-publico/agenda-municipal##Documentacion"/>
</rdf:Description>

<rdf:Description rdf:about="http://vocab.linkeddata.es/datosabiertos/def/sector-publico/agenda-municipal##Evento">
	<rdfs:subClassOf rdf:nodeID="genid48"/>
</rdf:Description>

<rdf:Description rdf:nodeID="genid48">
	<rdf:type rdf:resource="http://www.w3.org/2002/07/owl#Restriction"/>
	<owl:onProperty rdf:resource="http://vocab.linkeddata.es/datosabiertos/def/sector-publico/agenda-municipal##tipoEvento"/>
	<owl:allValuesFrom rdf:resource="http://www.w3.org/2004/02/skos/core#Concept"/>
</rdf:Description>

<rdf:Description rdf:about="http://vocab.linkeddata.es/datosabiertos/def/sector-publico/agenda-municipal##Evento">
	<rdfs:comment xml:lang="en">Action scheduled to take place at a certain date, time and place.</rdfs:comment>
	<rdfs:comment xml:lang="es">Suceso programado para realizarse en una determinada fecha, hora, y lugar.</rdfs:comment>
	<rdfs:isDefinedBy>http://vocab.linkeddata.es/datosabiertos/def/sector-publico/agenda-municipal</rdfs:isDefinedBy>
	<rdfs:label xml:lang="en">Event in agenda</rdfs:label>
	<rdfs:label xml:lang="es">Evento en agenda</rdfs:label>
</rdf:Description>
<!--  -->
<!-- http://vocab.linkeddata.es/datosabiertos/def/sector-publico/agenda-municipal##RolIntegranteEvento -->

<rdf:Description rdf:about="http://vocab.linkeddata.es/datosabiertos/def/sector-publico/agenda-municipal##RolIntegranteEvento">
	<rdf:type rdf:resource="http://www.w3.org/2002/07/owl#Class"/>
	<rdfs:subClassOf rdf:nodeID="genid49"/>
</rdf:Description>

<rdf:Description rdf:nodeID="genid49">
	<owl:intersectionOf rdf:nodeID="genid52"/>
</rdf:Description>

<rdf:Description rdf:nodeID="genid52">
	<rdf:type rdf:resource="http://www.w3.org/1999/02/22-rdf-syntax-ns#List"/>
	<rdf:first rdf:nodeID="genid53"/>
</rdf:Description>

<rdf:Description rdf:nodeID="genid53">
	<rdf:type rdf:resource="http://www.w3.org/2002/07/owl#Restriction"/>
	<owl:onProperty rdf:resource="http://vocab.linkeddata.es/datosabiertos/def/sector-publico/agenda-municipal##evento"/>
	<owl:allValuesFrom rdf:resource="http://vocab.linkeddata.es/datosabiertos/def/sector-publico/agenda-municipal##Evento"/>
</rdf:Description>

<rdf:Description rdf:nodeID="genid52">
	<rdf:rest rdf:nodeID="genid50"/>
</rdf:Description>

<rdf:Description rdf:nodeID="genid50">
	<rdf:type rdf:resource="http://www.w3.org/1999/02/22-rdf-syntax-ns#List"/>
	<rdf:first rdf:nodeID="genid51"/>
</rdf:Description>

<rdf:Description rdf:nodeID="genid51">
	<rdf:type rdf:resource="http://www.w3.org/2002/07/owl#Restriction"/>
	<owl:onProperty rdf:resource="http://vocab.linkeddata.es/datosabiertos/def/sector-publico/agenda-municipal##evento"/>
	<owl:qualifiedCardinality rdf:datatype="http://www.w3.org/2001/XMLSchema#nonNegativeInteger">1</owl:qualifiedCardinality>
	<owl:onClass rdf:resource="http://vocab.linkeddata.es/datosabiertos/def/sector-publico/agenda-municipal##Evento"/>
</rdf:Description>

<rdf:Description rdf:nodeID="genid50">
	<rdf:rest rdf:resource="http://www.w3.org/1999/02/22-rdf-syntax-ns#nil"/>
</rdf:Description>

<rdf:Description rdf:nodeID="genid49">
	<rdf:type rdf:resource="http://www.w3.org/2002/07/owl#Class"/>
</rdf:Description>

<rdf:Description rdf:about="http://vocab.linkeddata.es/datosabiertos/def/sector-publico/agenda-municipal##RolIntegranteEvento">
	<rdfs:subClassOf rdf:nodeID="genid54"/>
</rdf:Description>

<rdf:Description rdf:nodeID="genid54">
	<owl:intersectionOf rdf:nodeID="genid57"/>
</rdf:Description>

<rdf:Description rdf:nodeID="genid57">
	<rdf:type rdf:resource="http://www.w3.org/1999/02/22-rdf-syntax-ns#List"/>
	<rdf:first rdf:nodeID="genid58"/>
</rdf:Description>

<rdf:Description rdf:nodeID="genid58">
	<rdf:type rdf:resource="http://www.w3.org/2002/07/owl#Restriction"/>
	<owl:onProperty rdf:resource="http://vocab.linkeddata.es/datosabiertos/def/sector-publico/agenda-municipal##integra"/>
	<owl:allValuesFrom rdf:resource="http://xmlns.com/foaf/0.1/Agent"/>
</rdf:Description>

<rdf:Description rdf:nodeID="genid57">
	<rdf:rest rdf:nodeID="genid55"/>
</rdf:Description>

<rdf:Description rdf:nodeID="genid55">
	<rdf:type rdf:resource="http://www.w3.org/1999/02/22-rdf-syntax-ns#List"/>
	<rdf:first rdf:nodeID="genid56"/>
</rdf:Description>

<rdf:Description rdf:nodeID="genid56">
	<rdf:type rdf:resource="http://www.w3.org/2002/07/owl#Restriction"/>
	<owl:onProperty rdf:resource="http://vocab.linkeddata.es/datosabiertos/def/sector-publico/agenda-municipal##integra"/>
	<owl:qualifiedCardinality rdf:datatype="http://www.w3.org/2001/XMLSchema#nonNegativeInteger">1</owl:qualifiedCardinality>
	<owl:onClass rdf:resource="http://xmlns.com/foaf/0.1/Agent"/>
</rdf:Description>

<rdf:Description rdf:nodeID="genid55">
	<rdf:rest rdf:resource="http://www.w3.org/1999/02/22-rdf-syntax-ns#nil"/>
</rdf:Description>

<rdf:Description rdf:nodeID="genid54">
	<rdf:type rdf:resource="http://www.w3.org/2002/07/owl#Class"/>
</rdf:Description>

<rdf:Description rdf:about="http://vocab.linkeddata.es/datosabiertos/def/sector-publico/agenda-municipal##RolIntegranteEvento">
	<rdfs:subClassOf rdf:nodeID="genid59"/>
</rdf:Description>

<rdf:Description rdf:nodeID="genid59">
	<owl:intersectionOf rdf:nodeID="genid62"/>
</rdf:Description>

<rdf:Description rdf:nodeID="genid62">
	<rdf:type rdf:resource="http://www.w3.org/1999/02/22-rdf-syntax-ns#List"/>
	<rdf:first rdf:nodeID="genid63"/>
</rdf:Description>

<rdf:Description rdf:nodeID="genid63">
	<rdf:type rdf:resource="http://www.w3.org/2002/07/owl#Restriction"/>
	<owl:onProperty rdf:resource="http://vocab.linkeddata.es/datosabiertos/def/sector-publico/agenda-municipal##rol"/>
	<owl:allValuesFrom rdf:resource="http://www.w3.org/2004/02/skos/core#Concept"/>
</rdf:Description>

<rdf:Description rdf:nodeID="genid62">
	<rdf:rest rdf:nodeID="genid60"/>
</rdf:Description>

<rdf:Description rdf:nodeID="genid60">
	<rdf:type rdf:resource="http://www.w3.org/1999/02/22-rdf-syntax-ns#List"/>
	<rdf:first rdf:nodeID="genid61"/>
</rdf:Description>

<rdf:Description rdf:nodeID="genid61">
	<rdf:type rdf:resource="http://www.w3.org/2002/07/owl#Restriction"/>
	<owl:onProperty rdf:resource="http://vocab.linkeddata.es/datosabiertos/def/sector-publico/agenda-municipal##rol"/>
	<owl:qualifiedCardinality rdf:datatype="http://www.w3.org/2001/XMLSchema#nonNegativeInteger">1</owl:qualifiedCardinality>
	<owl:onClass rdf:resource="http://www.w3.org/2004/02/skos/core#Concept"/>
</rdf:Description>

<rdf:Description rdf:nodeID="genid60">
	<rdf:rest rdf:resource="http://www.w3.org/1999/02/22-rdf-syntax-ns#nil"/>
</rdf:Description>

<rdf:Description rdf:nodeID="genid59">
	<rdf:type rdf:resource="http://www.w3.org/2002/07/owl#Class"/>
</rdf:Description>

<rdf:Description rdf:about="http://vocab.linkeddata.es/datosabiertos/def/sector-publico/agenda-municipal##RolIntegranteEvento">
	<rdfs:comment xml:lang="es">Rol que tiene el integrante de un evento como asistente, convocante o titular.</rdfs:comment>
	<rdfs:comment xml:lang="en">Role that the member of an event has as assistant, chair or organizer.</rdfs:comment>
	<rdfs:isDefinedBy>http://vocab.linkeddata.es/datosabiertos/def/sector-publico/agenda-municipal</rdfs:isDefinedBy>
	<rdfs:label xml:lang="es">Rol integrante del evento</rdfs:label>
	<rdfs:label xml:lang="en">Role member of event</rdfs:label>
</rdf:Description>
<!--  -->
<!-- http://vocab.linkeddata.es/datosabiertos/def/sector-publico/territorio#Distrito -->

<rdf:Description rdf:about="http://vocab.linkeddata.es/datosabiertos/def/sector-publico/territorio#Distrito">
	<rdf:type rdf:resource="http://www.w3.org/2002/07/owl#Class"/>
	<rdfs:subClassOf rdf:resource="http://dbpedia.org/ontology/District"/>
	<terms:issued xml:lang="es">2014-03-28</terms:issued>
	<rdfs:comment xml:lang="es">Un distrito es cada una de las demarcaciones en que se subdivide un territorio o una población para distribuir y ordenar el ejercicio de los derechos civiles y políticos, o de las funciones públicas, o de los servicios administrativos [fuente: Diccionario de la Real Academia (DRAE) 2011]</rdfs:comment>
	<rdfs:isDefinedBy xml:lang="es">http://vocab.linkeddata.es/datosabiertos/def/sector-publico/territorio</rdfs:isDefinedBy>
	<rdfs:label xml:lang="es">Distrito</rdfs:label>
</rdf:Description>
<!--  -->
<!-- http://vocab.linkeddata.es/datosabiertos/def/sector-publico/territorio#Municipio -->

<rdf:Description rdf:about="http://vocab.linkeddata.es/datosabiertos/def/sector-publico/territorio#Municipio">
	<rdf:type rdf:resource="http://www.w3.org/2002/07/owl#Class"/>
	<rdfs:subClassOf rdf:resource="http://dbpedia.org/ontology/Municipality"/>
	<terms:issued>2014-03-28</terms:issued>
	<rdfs:comment xml:lang="es">Un Municipio es el ente local definido en el artículo 140 de la Constitución española y la entidad básica de la organización territorial del Estado según el artículo 1 de la Ley 7/1985, de 2 de abril, Reguladora de las Bases del Régimen Local. Tiene personalidad jurídica y plena capacidad para el cumplimiento de sus fines. La delimitación territorial de Municipio está recogida del REgistro Central de Cartografía del IGN.
Su nombre, que se especifica con la propiedad dct:title, es el proporcionado por el Registro de Entidades Locales del Ministerio de Política Territorial, en http://www.ine.es/nomen2/index.do</rdfs:comment>
	<rdfs:isDefinedBy rdf:resource="http://purl.org/derecho/vocabulario"/>
	<rdfs:isDefinedBy rdf:resource="http://vocab.linkeddata.es/datosabiertos/def/sector-publico/territorio"/>
	<rdfs:isDefinedBy rdf:resource="http://www.ign.es/ign/resources/acercaDe/tablon/ModeloDireccionesAGE.pdf‎"/>
	<rdfs:label xml:lang="es">Municipio</rdfs:label>
	<rdfs:seeAlso rdf:resource="http://purl.org/derecho/vocabulario#Municipio"/>
</rdf:Description>
<!--  -->
<!-- http://vocab.linkeddata.es/datosabiertos/def/urbanismo-infraestructuras/equipamiento#Equipamiento -->

<rdf:Description rdf:about="http://vocab.linkeddata.es/datosabiertos/def/urbanismo-infraestructuras/equipamiento#Equipamiento">
	<rdf:type rdf:resource="http://www.w3.org/2002/07/owl#Class"/>
	<rdfs:subClassOf rdf:resource="http://schema.org/Place"/>
	<rdfs:comment xml:lang="es">Equipamientos a los que un ciudadano puede acudir pertenecientes a una administración.</rdfs:comment>
	<rdfs:comment xml:lang="en">Equipment to which a citizen can access belonging to an administration.</rdfs:comment>
	<rdfs:isDefinedBy xml:lang="en">http://vocab.linkeddata.es/datosabiertos/def/urbanismo-infraestructura/equipamiento-municipal</rdfs:isDefinedBy>
	<rdfs:label xml:lang="es">equipamiento</rdfs:label>
	<rdfs:label xml:lang="en">equipment</rdfs:label>
</rdf:Description>
<!--  -->
<!-- http://www.w3.org/2004/02/skos/core#Concept -->

<rdf:Description rdf:about="http://www.w3.org/2004/02/skos/core#Concept">
	<rdf:type rdf:resource="http://www.w3.org/2002/07/owl#Class"/>
	<owl:disjointWith rdf:resource="http://www.w3.org/2004/02/skos/core#ConceptScheme"/>
	<terms:issued>2008-05-xx</terms:issued>
	<rdfs:isDefinedBy>http://www.w3.org/2008/05/skos</rdfs:isDefinedBy>
	<rdfs:label xml:lang="en">Concept</rdfs:label>
	<skos:definition xml:lang="en">An abstract idea or notion; a unit of thought.</skos:definition>
</rdf:Description>
<!--  -->
<!-- http://www.w3.org/2004/02/skos/core#ConceptScheme -->

<rdf:Description rdf:about="http://www.w3.org/2004/02/skos/core#ConceptScheme">
	<rdf:type rdf:resource="http://www.w3.org/2002/07/owl#Class"/>
	<terms:issued xml:lang="en">2008-05-xx</terms:issued>
	<rdfs:comment xml:lang="en">A concept scheme may be defined to include concepts from different sources.</rdfs:comment>
	<rdfs:comment xml:lang="en">Thesauri, classification schemes, subject heading lists, taxonomies, 'folksonomies', and other types of controlled vocabulary are all examples of concept schemes.  Concept schemes are also embedded in glossaries and terminologies.</rdfs:comment>
	<rdfs:isDefinedBy xml:lang="en">http://www.w3.org/2008/05/skos</rdfs:isDefinedBy>
	<rdfs:label xml:lang="en">Concept Scheme</rdfs:label>
	<skos1:definition xml:lang="en">A set of concepts, optionally including statements about semantic relationships between those concepts.</skos1:definition>
</rdf:Description>
<!--  -->
<!-- http://www.w3.org/ns/org#Membership -->

<rdf:Description rdf:about="http://www.w3.org/ns/org#Membership">
	<rdf:type rdf:resource="http://www.w3.org/2002/07/owl#Class"/>
	<owl:disjointWith rdf:resource="http://www.w3.org/ns/org#Organization"/>
	<owl:disjointWith rdf:resource="http://www.w3.org/ns/org#Role"/>
	<rdfs:comment xml:lang="en">Indicates the nature of an Agent's membership of an organization. Represents an n-ary relation between an Agent, an Organization and a Role. It is possible to directly indicate membership, independent of the specific Role, through use of the `org:memberOf` property.</rdfs:comment>
	<rdfs:comment xml:lang="es">Pertenencia o afiliación de un agente a una organización. Es una relación n-aria entre un agente, una organización y una actividad. Es posible indicar pertenencia mediante el uso de la propiedad `org:memberOf`, independientemente de la actividad específica que se desempeñe.</rdfs:comment>
	<rdfs:isDefinedBy>http://www.w3.org/ns/org</rdfs:isDefinedBy>
	<rdfs:label xml:lang="en">membership</rdfs:label>
	<rdfs:label xml:lang="es">membresía</rdfs:label>
</rdf:Description>
<!--  -->
<!-- http://www.w3.org/ns/org#Organization -->

<rdf:Description rdf:about="http://www.w3.org/ns/org#Organization">
	<rdf:type rdf:resource="http://www.w3.org/2002/07/owl#Class"/>
	<rdfs:subClassOf rdf:resource="http://xmlns.com/foaf/0.1/Agent"/>
	<owl:disjointWith rdf:resource="http://www.w3.org/ns/org#Role"/>
	<owl:disjointWith rdf:resource="http://xmlns.com/foaf/0.1/Group"/>
	<owl:disjointWith rdf:resource="http://xmlns.com/foaf/0.1/Person"/>
	<rdfs:comment xml:lang="es">Grupo de personas que se organiza en una comunidad u otro tipo de estructura social, comercial o política. Dicho grupo tiene un objetivo o motivo común para su existencia que va más allá del conjunto de personas que lo forman y que puede actuar como “agente”. A menudo las organizaciones se pueden agrupar en estructuras jerárquicas.</rdfs:comment>
	<rdfs:comment xml:lang="en">Represents a collection of people organized together into a community or other social, commercial or political structure. The group has some common purpose or reason for existence which goes beyond the set of people belonging to it and can act as an Agent. Organizations are often decomposable into hierarchical structures.</rdfs:comment>
	<rdfs:isDefinedBy rdf:resource="http://www.w3.org/ns/org"/>
	<rdfs:label xml:lang="en">Organization</rdfs:label>
	<rdfs:label xml:lang="es">organización</rdfs:label>
</rdf:Description>
<!--  -->
<!-- http://www.w3.org/ns/org#Role -->

<rdf:Description rdf:about="http://www.w3.org/ns/org#Role">
	<rdf:type rdf:resource="http://www.w3.org/2002/07/owl#Class"/>
	<rdfs:subClassOf rdf:resource="http://www.w3.org/2004/02/skos/core#Concept"/>
	<rdfs:comment xml:lang="en">Denotes a role that a Person or other Agent can take in an organization. Instances of this class describe the abstract role; to denote a specific instance of a person playing that role in a specific organization use an instance of `org:Membership`. It is common for roles to be arranged in some taxonomic structure and we use SKOS to represent that. The normal SKOS lexical properties should be used when labelling the Role. Additional descriptive properties for the Role, such as a Salary band, may be added by extension vocabularies.</rdfs:comment>
	<rdfs:comment xml:lang="es">Función que una persona o agente desempeña en el seno de una organización. Las instancias de esta clase describen la actividad en abstracto; si lo que se pretende es incluir una instancia que refleje la función o actividad que desempeña una persona en concreto en una organización específica, se indica el uso de instancias de la clase `org:Membership`. Es común que dichas actividades se representen en una estructura taxonómica mediante SKOS. Las propiedades léxicas de SKOS deberían utilizarse a la hora de denominar o etiquetar la actividad desempeñada. Para añadir propiedades descriptivas adicionales, como rango salarial, se tendrá que recurrir a vocabularios externos.</rdfs:comment>
	<rdfs:isDefinedBy>http://www.w3.org/ns/org</rdfs:isDefinedBy>
	<rdfs:label xml:lang="es">actividad</rdfs:label>
	<rdfs:label xml:lang="en">role</rdfs:label>
</rdf:Description>
<!--  -->
<!-- http://xmlns.com/foaf/0.1/Agent -->

<rdf:Description rdf:about="http://xmlns.com/foaf/0.1/Agent">
	<rdf:type rdf:resource="http://www.w3.org/2002/07/owl#Class"/>
	<rdfs:comment xml:lang="en">An agent (eg. person, group, software or physical artifact).</rdfs:comment>
	<rdfs:label xml:lang="en">Agent</rdfs:label>
</rdf:Description>
<!--  -->
<!-- http://xmlns.com/foaf/0.1/Group -->

<rdf:Description rdf:about="http://xmlns.com/foaf/0.1/Group">
	<rdf:type rdf:resource="http://www.w3.org/2002/07/owl#Class"/>
	<rdfs:subClassOf rdf:resource="http://xmlns.com/foaf/0.1/Agent"/>
	<owl:disjointWith rdf:resource="http://xmlns.com/foaf/0.1/Person"/>
	<rdfs:comment xml:lang="en">A class of Agents.</rdfs:comment>
	<rdfs:label xml:lang="en">Group</rdfs:label>
</rdf:Description>
<!--  -->
<!-- http://xmlns.com/foaf/0.1/Person -->

<rdf:Description rdf:about="http://xmlns.com/foaf/0.1/Person">
	<rdf:type rdf:resource="http://www.w3.org/2002/07/owl#Class"/>
	<rdfs:subClassOf rdf:resource="http://xmlns.com/foaf/0.1/Agent"/>
	<rdfs:comment xml:lang="en">A person.</rdfs:comment>
	<rdfs:isDefinedBy>http://xmlns.com/foaf/0.1/</rdfs:isDefinedBy>
	<rdfs:label xml:lang="en">Person</rdfs:label>
</rdf:Description>
<!--  -->
<!--  -->
<!--  -->
<!-- ################################################################# -->
<!-- # -->
<!-- #    Individuals -->
<!-- # -->
<!-- ################################################################# -->
<!--  -->
<!--  -->
<!-- http://vocab.linkeddata.es/datosabiertos/kos/sector-publico/agenda-municipal/canal -->

<rdf:Description rdf:about="http://vocab.linkeddata.es/datosabiertos/kos/sector-publico/agenda-municipal/canal">
	<rdf:type rdf:resource="http://www.w3.org/2002/07/owl#NamedIndividual"/>
	<rdf:type rdf:resource="http://www.w3.org/2004/02/skos/core#ConceptScheme"/>
</rdf:Description>
<!--  -->
<!-- http://vocab.linkeddata.es/datosabiertos/kos/sector-publico/agenda-municipal/rol -->

<rdf:Description rdf:about="http://vocab.linkeddata.es/datosabiertos/kos/sector-publico/agenda-municipal/rol">
	<rdf:type rdf:resource="http://www.w3.org/2002/07/owl#NamedIndividual"/>
	<rdf:type rdf:resource="http://www.w3.org/2004/02/skos/core#ConceptScheme"/>
</rdf:Description>
<!--  -->
<!-- http://vocab.linkeddata.es/datosabiertos/kos/sector-publico/agenda-municipal/tipo-acceso -->

<rdf:Description rdf:about="http://vocab.linkeddata.es/datosabiertos/kos/sector-publico/agenda-municipal/tipo-acceso">
	<rdf:type rdf:resource="http://www.w3.org/2002/07/owl#NamedIndividual"/>
	<rdf:type rdf:resource="http://www.w3.org/2004/02/skos/core#ConceptScheme"/>
</rdf:Description>
<!--  -->
<!-- http://vocab.linkeddata.es/datosabiertos/kos/sector-publico/agenda-municipal/tipo-evento -->

<rdf:Description rdf:about="http://vocab.linkeddata.es/datosabiertos/kos/sector-publico/agenda-municipal/tipo-evento">
	<rdf:type rdf:resource="http://www.w3.org/2002/07/owl#NamedIndividual"/>
	<rdf:type rdf:resource="http://www.w3.org/2004/02/skos/core#ConceptScheme"/>
</rdf:Description>
<!--  -->
<!-- http://vocab.linkeddata.es/datosabiertos/kos/sector-publico/agenda-municipal/tipo-sesion -->

<rdf:Description rdf:about="http://vocab.linkeddata.es/datosabiertos/kos/sector-publico/agenda-municipal/tipo-sesion">
	<rdf:type rdf:resource="http://www.w3.org/2002/07/owl#NamedIndividual"/>
	<rdf:type rdf:resource="http://www.w3.org/2004/02/skos/core#ConceptScheme"/>
</rdf:Description>
<!--  -->
<!-- Generated by the OWL API (version 4.2.8.20170104-2310) https://github.com/owlcs/owlapi -->

</rdf:RDF>